SystemF2: use rrwrite tactic to cleanup lifting lemmas

proof/DDC/Language/SystemF2/TySubst.v
@@ -30,9 +30,10 @@ Fixpoint substTTs (d: nat) (us: list ty) (tt: ty) :=
  match us with
  | nil      => tt
  | u :: us' => substTTs d us' 
-                 (substTT d (liftTT (List.length us') 0 u)
-                            tt)
+                 (substTT d u tt)
  end.
+
+
 
 
 (********************************************************************)
@@ -65,28 +66,23 @@ Proof.
 Qed.
 
 
+(********************************************************************)
 (* Lifting after substitution *)
-Lemma liftTT_substTT1
+Lemma liftTT_substTT_1
  :  forall n n' t1 t2
  ,  liftTT 1 n (substTT (n + n') t2 t1)
  =  substTT (1 + n + n') (liftTT 1 n t2) (liftTT 1 n t1).
 Proof.
  intros. gen n n' t2.
- induction t1; intros; simpl; try burn.
+ induction t1; intros; simpl; try burn; try (repeat rewritess).
 
  Case "TVar".
   repeat (simpl; fbreak_nat_compare; 
-          try lift_cases; try intros);
-   burn.
+          try lift_cases; try intros); burn.
 
  Case "TForall".
-  simpl.
-  rewrite (IHt1 (S n) n'). simpl.
-  rewrite (liftTT_liftTT' 0 n). auto.
-
- Case "TApp".
-  rewrite IHt1_1. 
-  rewrite IHt1_2. auto.
+  rewrite (IHt1 (S n) n').
+  rewrite (liftTT_liftTT_11 0 n). auto.
 Qed.
 
 
@@ -96,73 +92,69 @@ Lemma liftTT_substTT
  =  substTT (m + n + n') (liftTT m n t2) (liftTT m n t1).
 Proof.
  intros. gen n n'.
- induction m; intros.
-  simpl.  
-   rewrite liftTT_zero.
-   rewrite liftTT_zero.
-   rewrite liftTT_zero.
-   auto.
-  simpl.
-   assert (S m = 1 + m). 
-    omega. rewrite H.
-   rewrite <- liftTT_plus.
-   rewrite IHm.
-   assert (m + n + n' = n + (m + n')).
-    omega. rewrite H0.
-   rewrite liftTT_substTT1.
-   simpl. 
-   f_equal; rewrite liftTT_plus; auto.
+ induction m; intros; simpl.
+  repeat (rewrite liftTT_zero); auto.
+
+  rrwrite (S m = 1 + m).
+  rewrite <- liftTT_plus.
+  rewrite IHm.
+  rrwrite (m + n + n' = n + (m + n')).
+  rewrite liftTT_substTT_1. 
+  simpl; f_equal; rewrite liftTT_plus; auto.
 Qed.
 
 
+(* proof of this is probably too much of a hassle with the
+   inductive version of simultaneous substitution.
+   Do real simultaneous substitution taking a list of things
+   to substitute. 
+ *)
+Lemma liftTT_substTTs
+ :  forall m n n' ts t
+ ,  liftTT m n (substTTs (n + n') ts t)
+ =  substTTs (m + n + n') (map (liftTT m n) ts) (liftTT m n t).
+Proof.
+ intros. gen m n n' t. 
+ induction ts; intros.
+ 
+  simpl. auto.
+  simpl.
+
+  rewrite IHts.
+  rewrite liftTT_substTT.
+  rrwrite (n = n + 0).  
+  auto.
+Qed. 
+
+
+(********************************************************************)
+(*
 Lemma substTTs_TForall
  :  forall ts d t
  ,  substTTs d ts (TForall t)
  =  TForall (substTTs (1 + d) (map (liftTT 1 0) ts) t).
 Proof.
  intros. gen d t.
- induction ts; intros.
-  simpl. auto.
-  simpl.
-  rewrite map_length.
-   rewrite <- IHts.
-   f_equal. f_equal. f_equal.
-   rewrite liftTT_comm. auto.
-Qed.
-
-(*
-Lemma liftTT_substTTs
- :  forall m n n' ts t
- ,  liftTT m n (substTTs (n + n') ts t)
- =  substTTs (m + n + n') (map (liftTT m n) ts) (liftTT m n t).
-Proof.
- intros. gen m n n' ts.
- induction t; intros.
-
- Case "TCon".
-  induction ts.
-   auto.
-   simpl. rewrite IHts. auto.
-
- Case "TVar".
-   admit.
+ induction ts; intros; simpl; try burn.
 
  Case "TForall".
-  simpl.
-  rewrite substTTs_TForall. simpl.
-  rewrite substTTs_TForall. simpl.
-  f_equal.
-  assert (S (n + n') = S n + n').
-   omega. rewrite H.
-  rewrite IHt.
-  f_equal. omega. simpl.
-  rewrite map_map. rewrite map_map.
-  unfold compose.
-  f_equal.
-   extensionality x.
-   simpl.
+  rewrite map_length.
+  rewrite <- IHts.
+  rewrite liftTT_comm. auto.
+Qed.
 
+
+Lemma substTTs_TApp
+ :  forall ts d t1 t2
+ ,  substTTs d ts (TApp t1 t2)
+ =  TApp (substTTs d ts t1) (substTTs d ts t2).
+Proof.
+ intros. gen d t1 t2.
+ induction ts; intros; simpl; try burn.
+Qed.
 *)
+(********************************************************************)
+
 
 Lemma liftTT_substTT'
  :  forall n n' t1 t2
@@ -170,25 +162,21 @@ Lemma liftTT_substTT'
  =  substTT n (liftTT 1 (n + n') t2) (liftTT 1 (1 + n + n') t1).
 Proof.
  intros. gen n n' t2.
- induction t1; intros; eauto.
+ induction t1; intros; try (repeat rewritess); eauto.
 
  Case "TVar".
   repeat ( unfold liftTT; unfold substTT; fold liftTT; fold substTT
-         ; try lift_cases; try fbreak_nat_compare
+         ; try lift_cases
+         ; try fbreak_nat_compare
          ; intros); try burn.
 
  Case "TForall".
-  simpl. f_equal.
-  rewrite (IHt1 (S n) n'). f_equal.
-   simpl. rewrite (liftTT_liftTT' 0 (n + n')). auto.
-
- Case "TApp".
-  simpl. f_equal.
-   apply IHt1_1.
-   apply IHt1_2.
+  simpl. rewrite (IHt1 (S n) n').
+  simpl. rewrite (liftTT_liftTT_11 0 (n + n')). auto.
 Qed.
 
 
+(********************************************************************)
 (* Commuting substitutions. *)
 Lemma substTT_substTT
  :  forall n m t1 t2 t3
@@ -197,7 +185,7 @@ Lemma substTT_substTT
               (substTT (1 + n + m) (liftTT 1 n t3) t1).
 Proof.
  intros. gen n m t2 t3.
- induction t1; intros; auto.
+ induction t1; intros; eauto.
 
  Case "TVar".
   repeat (simpl; fbreak_nat_compare); try burn.
@@ -205,12 +193,14 @@ Proof.
 
  Case "TForall".
   simpl. f_equal.
-  rewrite (IHt1 (S n) m). f_equal.
-   simpl. rewrite (liftTT_substTT1 0 (n + m)). auto.
-   simpl. rewrite (liftTT_liftTT' 0 n). auto.  
+  rewrite (IHt1 (S n) m). 
+  f_equal; simpl.
+   rewrite (liftTT_substTT_1 0 (n + m)). auto.
+   rewrite (liftTT_liftTT_11 0 n). auto.  
 
  Case "TApp".
   simpl. f_equal.
    apply IHt1_1.
    apply IHt1_2.
 Qed.
+
